simlify

theories/SLFStruct.v
@@ -23,6 +23,29 @@ Implicit Type v : val.
 (* TODO: fix p+f to f+p *)
 (* TODO explain val_ptr_add and its spec *)
 
+(* TODO : limitation of xapp for lemmas with premises... *)
+
+Lemma length_zero_inv : forall A (L:list A),
+  length L = 0%nat ->
+  L = nil.
+Proof using.
+  introv N. destruct L as [|]; rew_list in *; tryfalse. eauto.
+Qed.
+
+Lemma length_one_inv : forall A (L:list A),
+  length L = 1%nat ->
+  exists x, L = x::nil.
+Proof using.
+  introv N. destruct L as [|x [|]]; rew_list in *; tryfalse. eauto.
+Qed.
+
+
+Lemma range_split : forall n,
+  n > 1 ->
+  0 < Z.quot n 2 < n.
+Admitted. (* TODO *)
+
+
 (* ####################################################### *)
 (* ####################################################### *)
 (* ####################################################### *)
@@ -119,6 +142,40 @@ Lemma harray_not_null : forall p L,
   harray L p ==> harray L p \* \[p <> null].
 Proof using. introv N. unfold harray. xsimpl*. Qed.
 
+(** The description of an array, that is, a set of consecutive cells,
+    can be split in two parts, at an arbitrary index. Concretely, if
+    we have [harray (L1++L2) p], then we can separate the left part
+    [harray L1 p] from the right part [harray L2 q], where the address
+    [q] is equal to [p + length L1]. Reciprocally, the two parts can
+    be merged back into the original form at any time. 
+
+    Note that the same property is true of the heap predicate [hcells]. *)
+
+Lemma hcells_concat_eq : forall p L1 L2,
+  hcells (L1++L2) p = (hcells L1 p \* hcells L2 (length L1 + p)%nat).
+Proof using.
+  intros. gen p. induction L1; intros; rew_list; simpl.
+  { xsimpl. }
+  { rewrite IHL1. math_rewrite (length L1 + S p = S (length L1 + p))%nat.
+    xsimpl. }
+Qed.
+
+Lemma harray_concat_eq : forall p L1 L2,
+  harray (L1++L2) p = (harray L1 p \* harray L2 (length L1 + p)%nat).
+Proof using.
+  intros. unfold harray, null, loc. rewrite hcells_concat_eq.
+  applys himpl_antisym; xsimpl*. math.
+Qed.
+
+(** Remark: this "splitting lemma for arrays" is useful to carry out local
+    reasoning on arrays, by focusing on the segment of the array involved
+    in each recursive call, and obtaining for free the fact that the
+    cells outside of the segment remain unmodified. *)
+
+
+(* ####################################################### *)
+(** ** Specification of the allocation of consecutive cells *)
+
 (** The operation [val_alloc k] allocates [k] consecutive cells. Let [p]
     denote the pointer returned. The allocated cells have addresses in
     the range from [p] inclusive to [p+k] exclusive. These cells have for
@@ -137,10 +194,6 @@ Parameter val_uninit : val.
 
 Definition harray_uninit (k:nat) (p:loc) : hprop :=
   harray (LibList.make k val_uninit) p.
-
-
-(* ####################################################### *)
-(** ** Specification of the allocation of consecutive cells *)
 
 (** Let us specify the behavior of the allocation function using a
     triple. We first state a specification with an argument of type [nat],
@@ -277,256 +330,64 @@ Qed.
 
 
 (* ####################################################### *)
-(** ** Reasoning about arrays *)
+(** ** Specification of array access operations *)
 
 Module Arrays.
-
-(** Array operations *)
-
 Import LibListZ.
-Implicit Types L : list val.
+Implicit Types L : list val. (* TODO *)
 
-(** [val_array_get p i] *)
+(** The operation [val_array_get p i] returns the contents of the [i]-th 
+    cell of the array at location [p]. *)
 
 Parameter val_array_get : val.
 
-Notation "'Array'' p `[ i ]" := (trm_app (trm_app (trm_val val_array_get) p) i)
-  (at level 69, p at level 0, no associativity,
-   format "'Array''  p `[ i ]") : charac.
+(** The specification of this operation involves the operation [list_get L i]
+    that returns the [i]-th element of a list of values. The TLC library
+    [LibListZ] provides a general-purpose formalization of this definition,
+    yet its presentation relies on typeclasses, whic are uncessarily complex
+    for our purposes here. To avoid this complexity, let us simply axiomatize
+    the operation. *)
 
-Lemma triple_array_get : forall p i L,
+Parameter list_get : list val -> int -> val.
+
+(** The specification of [val_array_get] is as follows. The precondition
+    describes the array in the form [harray L p], with a premise that
+    requires the index [i] to be in the valid range, that is, between
+    zero (inclusive) and the length of [L] (exclusive). The postcondition
+    asserts that the result value is [list_get L i], and mentions the
+    unmodified array, still described by [harray L p]. *)
+
+Parameter triple_array_get : forall p i L,
   0 <= i < length L ->
   triple (val_array_get p i)
     (harray L p)
-    (fun r => \[r = L[i]] \* harray L p).
-Admitted.
+    (fun r => \[r = list_get L i] \* harray L p).
 
-(** [val_array_set p i v] *)
+(** The operation [val_array_set p i v] updates the contents of the [i]-th 
+    cell of the array at location [p]. *)
 
 Parameter val_array_set : val.
 
-Notation "'Array'' p `[ i ] `<- x" := (trm_app (trm_app (trm_app (trm_val val_array_set) p) i) x)
-  (at level 69, p at level 0, no associativity,
-   format "'Array''  p `[ i ]  `<-  x") : charac.
+(** Again, for stating the specification, we axiomatize the corresponding 
+    operation on lists: [list_update L i v] describes the update to the
+    list [L] by replacing the value at index [i] with the value [v]. *)
 
-Lemma triple_array_set : forall p i v L,
+Parameter list_update : list val -> int -> val -> list val.
+
+(** The specification of [val_array_set] admits the same precondition as
+    [val_array_get], with [harray L p] and the constraint [0 <= i < length L].
+    Its postcondition describes the updated array using a predicate of the
+    form [harray L' p], where [L'] corresponds to [list_update L i v]. *)
+
+Parameter triple_array_set : forall p i v L,
   0 <= i < length L ->
   triple (val_array_set p i v)
     (harray L p)
-    (fun r => \[r = val_unit] \* harray (L[i:=v]) p).
-Admitted.
+    (fun _ => harray (list_update L i v) p).
 
-(** Example program
-
-[[
-    let rec array_incr p n =
-      if n > 0 then begin
-        p.(n-1) <- p.(n-1) + 1;
-        array_incr p (n-1)
-      end
-]]
-*)
-
-Import SLFProgramSyntax. (* TODO *)
-
-Definition array_incr : val :=
-  VFix 'f 'p 'n :=
-    Let 'b := ('n '> 0) in
-    If_ 'b Then
-      Let 'i := 'n '- 1 in
-      Let 'x := val_array_get 'p 'i in
-      Let 'y := 'x '+ 1 in
-      val_array_set 'p 'i 'y ';
-      'f 'p 'i
-    End.
-
-Definition harray_int (L:list int) (p:loc) : hprop :=
-  harray (LibList.map val_int L) p.
-
-Lemma triple_array_incr : forall (n:int) (L:list int) p,
-  n = LibListZ.length L ->
-  triple (array_incr p n)
-    (harray_int L p)
-    (fun _ => harray_int (LibList.map (fun x => x + 1) L) p).
-Proof using.
-  introv K. gen n. induction_wf IH: (@list_sub int) L. introv N. xwp.
-  skip. (* tODO *)
-Qed.
+Hint Resolve triple_array_get triple_array_set : triple.
 
 End Arrays.
-
-
-(* ####################################################### *)
-(** ** Local reasoning with arrays *)
-
-(** Consider the function [array_incr], which increments all the cells of
-    an array of integer by one unit.
-
-    An efficient, parallel version of this function can be implemented using
-    a divide-and-conquer approach: if the array has length more than [1],
-    then split in two parts and make a recursive call on each of the two parts.
-    The two recursive calls can be safely executed in parallel, because they
-    act over disjoint pieces of the array. Our programming language does not
-    enable us to express this form of parallelism, yet it would be possible
-    to do so using a simple extension based on the "fork-join" parallel construct.
-
-[[
-    let rec array_incr_par n p =
-      if n = 1 then incr p
-      else if n > 1 then
-        let m = n/2 in
-        array_incr_par x m;
-        array_incr_par x (n-m) (p+m)
-]]
-
-    Our concern here is to show how the description of an array can be split
-    in two parts in the course of a recursive function. *)
-
-(** The description of an array, that is, a set of consecutive cells,
-    can be split in two parts, at an arbitrary index. Concretely, if
-    we have [harray (L1++L2) p], then we can separate the left part
-    [harray L1 p] from the right part [harray L2 q], where the address
-    [q] is equal to [p + length L1]. Reciprocally, the two parts can
-    be merged back into the original form at any time. *)
-
-Lemma hcells_concat_eq : forall p L1 L2,
-  hcells (L1++L2) p = (hcells L1 p \* hcells L2 (length L1 + p)%nat).
-Proof using.
-  intros. gen p. induction L1; intros; rew_list; simpl.
-  { xsimpl. }
-  { rewrite IHL1. math_rewrite (length L1 + S p = S (length L1 + p))%nat.
-    xsimpl. }
-Qed.
-
-Lemma harray_concat_eq : forall p L1 L2,
-  harray (L1++L2) p = (harray L1 p \* harray L2 (length L1 + p)%nat).
-Proof using.
-  intros. unfold harray, null, loc. rewrite hcells_concat_eq.
-  applys himpl_antisym; xsimpl*. math.
-Qed.
-
-(** To deal with the base cases, the following two lemmas are helpul. *)
-
-Lemma hcells_nil_eq : forall p,
-  hcells nil p = \[].
-Proof using. auto. Qed.
-
-Lemma hcells_one_eq : forall p x,
-  hcells (x::nil) p = (p ~~> x).
-Proof using. intros. simpl. xsimpl*. Qed.
-
-Lemma harray_nil_eq : forall p,
-  harray nil p = \[p <> null].
-Proof using. intros. unfold harray. rewrite hcells_nil_eq. xsimpl*. Qed.
-
-Lemma harray_one_eq : forall p x,
-  harray (x::nil) p = (p ~~> x).
-Proof using.
-  intros. unfold harray. rewrite hcells_one_eq. applys himpl_antisym.
-  { xsimpl. } { xchanges hsingle_not_null. }
-Qed.
-
-(** Let us put this lemma to practice on our example program. *)
-
-Import DemoPrograms.
-
-Definition array_incr_par : val :=
-  VFix 'f 'p 'n :=
-    Let 'b1 := ('n '= 1) in
-    If_ 'b1 Then incr 'p Else
-    Let 'b2 := ('n '> 1) in
-    If_ 'b2 Then
-      Let 'm := 'n '/ 2 in
-      Let 'n2 := ('n '- 'm) in
-      Let 'p2 := (val_ptr_add 'p 'm) in
-      'f 'p 'm ';
-      'f 'p2 'n2
-    End.
-
-Definition vals_of_ints (L:list int) : list val :=
-  LibList.map val_int L.
-
-Lemma length_one_inv : forall A (L:list A),
-  length L = 1%nat ->
-  exists x, L = x::nil.
-Proof using.
-  introv N. destruct L as [|x [|]]; rew_list in *; tryfalse. eauto.
-Qed.
-
-Lemma length_zero_inv : forall A (L:list A),
-  length L = 0%nat ->
-  L = nil.
-Proof using.
-  introv N. destruct L as [|]; rew_list in *; tryfalse. eauto.
-Qed.
-
-Lemma range_split : forall n,
-  n > 1 ->
-  0 < Z.quot n 2 < n.
-Admitted. (* TODO *)
-
-Parameter triple_div : forall n1 n2 : int,
-  triple (val_div n1 n2)
-    \[n2 <> 0]
-    (fun r => \[r = val_int (Z.quot n1 n2)]).
-
-Hint Resolve triple_div : triple.
-
-Definition harray_int (L:list int) (p:loc) : hprop :=
-  harray (LibList.map val_int L) p.
-
-Lemma harray_int_nil_eq : forall p,
-  harray_int nil p = \[p <> null].
-Proof using. intros. unfold harray_int. rew_listx. rewrite* harray_nil_eq. Qed.
-
-Lemma harray_int_one_eq : forall p n,
-  harray_int (n::nil) p = (p ~~> (val_int n)).
-Proof using. intros. unfold harray_int. rew_listx. rewrite* harray_one_eq. Qed.
-
-Lemma harray_int_concat_eq : forall p L1 L2,
-  harray_int (L1++L2) p = (harray_int L1 p \* harray_int L2 (length L1 + p)%nat).
-Proof using. intros. unfold harray_int. rew_listx. rewrite* harray_concat_eq. rew_listx*. Qed.
-
-Import LibListZ.
-Open Scope liblist_scope.
-Lemma take_app_drop_spec_nonneg : forall A (n:int) (l:list A),
-  0 <= n <= length l ->
-  exists f r,
-      l = f ++ r
-   /\ length f = n
-   /\ length r = length l - n.
-Proof using.
-  introv M. exists (take n l) (drop n l).
-  forwards* (R&_): take_app_drop_spec n l.
-Qed.
-
-
-Lemma triple_array_incr : forall (n:int) L p,
-  n = LibListZ.length L ->
-  triple (array_incr_par p n)
-    (harray_int L p)
-    (fun _ => harray_int (LibList.map (fun x => x + 1) L) p).
-Proof using.
-  intros n. induction_wf IH: (wf_downto 0) n.
-  introv E. xwp. xapp. xif; intros C1.
-  { forwards (x&Hx): length_one_inv L. math. (* TODO math *) subst.
-    rewrite harray_int_one_eq. xapp. rewrite <- harray_one_eq. xsimpl. }
-  { asserts C1': (n <> 1). { intros N. applys C1. fequals. } clear C1. (* TODO cleanup *)
-    xapp. xif; intros C2.
-    { forwards R: range_split n. { math. }
-      xapp. { math. } sets m: (Z.quot n 2).
-      xapp. xapp triple_ptr_add. { math. }
-      forwards (L1&L2&EL&LL1&LL2): take_app_drop_spec_nonneg m L. { math. }
-      rewrite EL. rewrite harray_int_concat_eq.
-      xapp (>> IH L1). { math. } { math. }
-      rew_listx. asserts_rewrite (abs (p + m) = (LibList.length L1 + p)%nat).
-      { apply eq_nat_of_eq_int. rewrite abs_nonneg; math. }
-      xapp (>> IH L2). { math. } { math. }
-      rewrite harray_int_concat_eq. rew_listx. xsimpl. }
-    { asserts En: (n = 0). { math. }
-      forwards HL: (length_zero_inv L). { math. }
-      xval. subst. do 2 rewrite harray_int_nil_eq. xsimpl*. } }
-Qed.
 
 
 (* ########################################################### *)
