extra/SLFArrayIncr.v
@@ -1,0 +1,241 @@
+
+(* ####################################################### *)
+(** ** Local reasoning with arrays *)
+
+(** Consider the function [array_incr], which increments all the cells of
+    an array of integer by one unit.
+
+    An efficient, parallel version of this function can be implemented using
+    a divide-and-conquer approach: if the array has length more than [1],
+    then split in two parts and make a recursive call on each of the two parts.
+    The two recursive calls can be safely executed in parallel, because they
+    act over disjoint pieces of the array. Our programming language does not
+    enable us to express this form of parallelism, yet it would be possible
+    to do so using a simple extension based on the "fork-join" parallel construct.
+
+[[
+    let rec array_incr_par n p =
+      if n = 1 then incr p
+      else if n > 1 then begin
+        let m = n/2 in
+        array_incr_par x m;
+        array_incr_par x (n-m) (p+m)
+      end
+]]
+
+    Our concern here is to show how the description of an array can be split
+    in two parts in the course of a recursive function. *)
+
+(** The description of an array, that is, a set of consecutive cells,
+    can be split in two parts, at an arbitrary index. Concretely, if
+    we have [harray (L1++L2) p], then we can separate the left part
+    [harray L1 p] from the right part [harray L2 q], where the address
+    [q] is equal to [p + length L1]. Reciprocally, the two parts can
+    be merged back into the original form at any time. *)
+
+Lemma hcells_concat_eq : forall p L1 L2,
+  hcells (L1++L2) p = (hcells L1 p \* hcells L2 (length L1 + p)%nat).
+Proof using.
+  intros. gen p. induction L1; intros; rew_list; simpl.
+  { xsimpl. }
+  { rewrite IHL1. math_rewrite (length L1 + S p = S (length L1 + p))%nat.
+    xsimpl. }
+Qed.
+
+Lemma harray_concat_eq : forall p L1 L2,
+  harray (L1++L2) p = (harray L1 p \* harray L2 (length L1 + p)%nat).
+Proof using.
+  intros. unfold harray, null, loc. rewrite hcells_concat_eq.
+  applys himpl_antisym; xsimpl*. math.
+Qed.
+
+(** To deal with the base cases, the following two lemmas are helpul. *)
+
+Lemma hcells_nil_eq : forall p,
+  hcells nil p = \[].
+Proof using. auto. Qed.
+
+Lemma hcells_one_eq : forall p x,
+  hcells (x::nil) p = (p ~~> x).
+Proof using. intros. simpl. xsimpl*. Qed.
+
+Lemma harray_nil_eq : forall p,
+  harray nil p = \[p <> null].
+Proof using. intros. unfold harray. rewrite hcells_nil_eq. xsimpl*. Qed.
+
+Lemma harray_one_eq : forall p x,
+  harray (x::nil) p = (p ~~> x).
+Proof using.
+  intros. unfold harray. rewrite hcells_one_eq. applys himpl_antisym.
+  { xsimpl. } { xchanges hsingle_not_null. }
+Qed.
+
+(** Let us put this lemma to practice on our example program. *)
+
+Import DemoPrograms.
+
+Definition array_incr_par : val :=
+  VFix 'f 'p 'n :=
+    Let 'b1 := ('n '= 1) in
+    If_ 'b1 Then incr 'p Else
+    Let 'b2 := ('n '> 1) in
+    If_ 'b2 Then
+      Let 'm := 'n '/ 2 in
+      Let 'n2 := ('n '- 'm) in
+      Let 'p2 := (val_ptr_add 'p 'm) in
+      'f 'p 'm ';
+      'f 'p2 'n2
+    End.
+
+Definition vals_of_ints (L:list int) : list val :=
+  LibList.map val_int L.
+
+Parameter triple_div : forall n1 n2 : int,
+  triple (val_div n1 n2)
+    \[n2 <> 0]
+    (fun r => \[r = val_int (Z.quot n1 n2)]).
+
+Hint Resolve triple_div : triple.
+
+Definition harray_int (L:list int) (p:loc) : hprop :=
+  harray (LibList.map val_int L) p.
+
+Lemma harray_int_nil_eq : forall p,
+  harray_int nil p = \[p <> null].
+Proof using. intros. unfold harray_int. rew_listx. rewrite* harray_nil_eq. Qed.
+
+Lemma harray_int_one_eq : forall p n,
+  harray_int (n::nil) p = (p ~~> (val_int n)).
+Proof using. intros. unfold harray_int. rew_listx. rewrite* harray_one_eq. Qed.
+
+Lemma harray_int_concat_eq : forall p L1 L2,
+  harray_int (L1++L2) p = (harray_int L1 p \* harray_int L2 (length L1 + p)%nat).
+Proof using. intros. unfold harray_int. rew_listx. rewrite* harray_concat_eq. rew_listx*. Qed.
+
+Import LibListZ.
+Open Scope liblist_scope.
+
+Lemma take_app_drop_spec_nonneg : forall A (n:int) (l:list A),
+  0 <= n <= length l ->
+  exists f r,
+      l = f ++ r
+   /\ length f = n
+   /\ length r = length l - n.
+Proof using.
+  introv M. exists (take n l) (drop n l).
+  forwards* (R&_): take_app_drop_spec n l.
+Qed.
+
+Lemma triple_array_incr : forall (n:int) L p,
+  n = LibListZ.length L ->
+  triple (array_incr_par p n)
+    (harray_int L p)
+    (fun _ => harray_int (LibList.map (fun x => x + 1) L) p).
+Proof using.
+  intros n. induction_wf IH: (wf_downto 0) n.
+  introv E. xwp. xapp. xif; intros C1.
+  { forwards (x&Hx): length_one_inv L. math. (* TODO math *) subst.
+    rewrite harray_int_one_eq. xapp. rewrite <- harray_one_eq. xsimpl. }
+  { asserts C1': (n <> 1). { intros N. applys C1. fequals. } clear C1. (* TODO cleanup *)
+    xapp. xif; intros C2.
+    { forwards R: range_split n. { math. }
+      xapp. { math. } sets m: (Z.quot n 2).
+      xapp. xapp triple_ptr_add. { math. }
+      forwards (L1&L2&EL&LL1&LL2): take_app_drop_spec_nonneg m L. { math. }
+      rewrite EL. rewrite harray_int_concat_eq.
+      xapp (>> IH L1). { math. } { math. }
+      rew_listx. asserts_rewrite (abs (p + m) = (LibList.length L1 + p)%nat).
+      { apply eq_nat_of_eq_int. rewrite abs_nonneg; math. }
+      xapp (>> IH L2). { math. } { math. }
+      rewrite harray_int_concat_eq. rew_listx. xsimpl. }
+    { asserts En: (n = 0). { math. }
+      forwards HL: (length_zero_inv L). { math. }
+      xval. subst. do 2 rewrite harray_int_nil_eq. xsimpl*. } }
+Qed.
+
+
+
+Notation "'Array'' p `[ i ]" := (trm_app (trm_app (trm_val val_array_get) p) i)
+  (at level 69, p at level 0, no associativity,
+   format "'Array''  p `[ i ]") : charac.
+
+Notation "'Array'' p `[ i ] `<- x" := (trm_app (trm_app (trm_app (trm_val val_array_set) p) i) x)
+  (at level 69, p at level 0, no associativity,
+   format "'Array''  p `[ i ]  `<-  x") : charac.
+
+
+
+
+(** Let us present the verification of an example program involving arrays.
+    The function [array_incr p n] increments by one unit the contents of
+    each of the [n] cells from the array at location [p].
+
+    It is implemented as a recursive function (because our language does not
+    feature for-loops). For simplicity of the code, it begins by incrementing
+    the cells near the end of the array, and decrements the value of the
+    argument [n] at each recursive call.
+
+[[
+    let rec array_incr p n =
+      if n > 0 then begin
+        p.(n-1) <- p.(n-1) + 1;
+        array_incr p (n-1)
+      end
+]]
+*)
+
+Import SLFProgramSyntax. (* TODO *)
+
+Definition array_incr : val :=
+  VFix 'f 'p 'n :=
+    Let 'b := ('n '> 0) in
+    If_ 'b Then
+      Let 'i := 'n '- 1 in
+      Let 'x := val_array_get 'p 'i in
+      Let 'y := 'x '+ 1 in
+      val_array_set 'p 'i 'y ';
+      'f 'p 'i
+    End.
+
+(** To specify the function [array_incr], we introduce an auxiliary definition
+    specialized for describing arrays of integers. The predicate [harray_int L p]
+    is similar to [harray L p] with the difference that [L] has type [list int]
+    instead of [list val]. *)
+
+Definition harray_int (L:list int) (p:loc) : hprop :=
+  harray (LibList.map val_int L) p.
+
+(** The specification of [array_incr] includes a precondition [harray_int L p],
+    and a postcondition of the form [harray_int L' p], where [L'] is obtained
+    by adding one unit to the every element from [L]. Formally, [L'] is equal to
+    [LibList.map (fun x => x + 1) L]. *)
+
+
+Implicit Types i : int. (* TODO *)
+
+Parameter triple_array_get' : forall p i L,
+  triple (val_array_get p i)
+    (harray L p \* \[0 <= i < length L])
+    (fun r => \[r = list_get L i] \* harray L p).
+
+Parameter triple_array_set': forall p i v L,
+  triple (val_array_set p i v)
+    (harray L p \* \[0 <= i < length L])
+    (fun _ => harray (list_update L i v) p).
+
+Hint Resolve triple_array_get' triple_array_set' : triple.
+
+Lemma triple_array_incr : forall (n:int) (L:list int) p,
+  n = LibListZ.length L ->
+  triple (array_incr p n)
+    (harray_int L p)
+    (fun _ => harray_int (LibList.map (fun x => x + 1) L) p).
+Proof using.
+  introv K. gen n. induction_wf IH: (@list_sub int) L. introv N. xwp.
+  xapp. xif; intros C.
+  { forwards (x&L'&->): length_pos_inv_last L. { math. } rew_listx in *.
+    xapp. xapp. { rewrite length_map. rew_listx. (* TODO rew_listx. *) math. }
+    rew_listx.
+    xapp. xapp triple_array_get. xapp_debug. eapply H.
+  { xval. rewrite (length_zero_inv L); [|math]. rew_listx. xsimpl. }
+Qed.
